rocq/definitions/Determinism.v
@@ -8,10 +8,8 @@ Module Type DeterminismDef (LD : LangDefs).
     Import LD.
     Import LangNotations.
     Section Determinism.
-        (* take this one as axiom *)
         Definition one_step_det cs :=
             forall cs1 cs2 a1 a2,
                 cs -->[a1] cs1 -> cs -->[a2] cs2 -> (a1 = a2) /\ (cs1 = cs2).
-        (* TODO: in addition to one step, prove that 2 finite traces produced from cs must be equal*)
     End Determinism.
 End DeterminismDef.
