rocq/theories/SecTheory.v
@@ -3,7 +3,7 @@ Require Import Lang.
 Require Import SecPol.
 Require Import Determinism.
 Require Import SecDef SecPol Trace.
-Require Import Grounding.
+Require Import BaseTheory.
 From Coq Require Import Equality Relations RelationClasses List Compare.
 Import ListNotations.
 
@@ -14,6 +14,22 @@ Module Type SecurityTheory (B : Basic) (LD : LangDefs) (TD : TraceDefs B LD) (SP
   Import LangNotations.
 
   Section SilentProperties.
+      Theorem silent_erasure : forall a l, sil a -> erase (a :: l) = erase l.
+        intros.
+        unfold erase.
+        destruct (sil_dec a).
+        - trivial.
+        - contradiction.
+      Qed.
+
+      Theorem non_silent_erasure : forall a l, ~ (sil a) -> erase (a :: l) = a :: (erase l).
+        intros.
+        unfold erase.
+        destruct (sil_dec a).
+        - contradiction.
+        - trivial.
+      Qed.
+
       Theorem silent_indistinct : forall c m a p, sil a -> Same_set Store (atk_knowledge c m p) (atk_knowledge c m (a :: p)).
         unfold Same_set, Included, In, atk_knowledge, deq_evt_lst.
         intros.
@@ -32,25 +48,77 @@ Module Type SecurityTheory (B : Basic) (LD : LangDefs) (TD : TraceDefs B LD) (SP
     End SilentProperties.
 
   Section DEqLists.
-    Theorem deq_evt_lst_refl : forall l1, 
-      deq_evt_lst l1 l1 -> deq_evt_lst l1 l1.
+    Theorem deq_evt_lst_refl : forall l1, deq_evt_lst l1 l1.
+      intros.
+      unfold deq_evt_lst.
       trivial.
     Qed.
 
-    Theorem deq_evt_lst_sym : forall l1 l2, 
-      deq_evt_lst l1 l2 -> deq_evt_lst l2 l1.
+    Theorem deq_evt_lst_sym : forall l1 l2,  deq_evt_lst l1 l2 -> deq_evt_lst l2 l1.
       unfold deq_evt_lst.
       intros.
       rewrite H.
       reflexivity.
     Qed.
 
-    Theorem deq_evt_lst_trans : forall l1 l2 l3,
-      deq_evt_lst l1 l2 -> deq_evt_lst l2 l3 -> deq_evt_lst l1 l3.
+    Theorem deq_evt_lst_trans : forall l1 l2 l3, deq_evt_lst l1 l2 -> deq_evt_lst l2 l3 -> deq_evt_lst l1 l3.
       unfold deq_evt_lst.
       intros.
       rewrite H, H0.
       reflexivity.
     Qed.
   End DEqLists.
+
+  Section DleLists.
+    Theorem dle_evt_lst_refl : forall l1, dle_evt_lst l1 l1.
+      intros.
+      unfold dle_evt_lst.
+      induction l1.
+        - auto.
+        - unfold erase.
+          destruct (sil_dec a); auto.
+    Qed.
+
+    Theorem dle_evt_lst_trans : forall l1 l2 l3, dle_evt_lst l1 l2 -> dle_evt_lst l2 l3 -> dle_evt_lst l1 l3.
+      unfold dle_evt_lst.
+      intros.
+      pose proof (@prefix_preorder_inst Event) as [_ Htrans].
+      unfold Transitive in Htrans.
+      apply (Htrans (erase l1) (erase l2) (erase l3)); assumption.
+    Qed.
+  End DleLists.
+
+  Section DeqTracePfx.
+    Instance deq_pfx_equiv : Equivalence deq_pfx.
+      destruct deq_store_equiv as [Hdsr Hdss Hdst].
+        split; unfold deq_pfx, Reflexive, Symmetric, Transitive.
+        - auto using deq_evt_lst_refl.
+        - intros [s1 l1] [s2 l2] [H1 H2].
+          auto using deq_evt_lst_sym.
+        - intros [s1 l1] [s2 l2] [s3 l3] [H1 H2] [H3 H4].
+          unfold Transitive in Hdst.
+          split.
+          + apply (deq_evt_lst_trans l1 l2 l3) in H1. 
+            * apply H1.
+            * apply H3.
+          + apply (Hdst s1 s2 s3) in H2.
+            * apply H2.
+            * apply H4.
+    Defined. 
+    
+    Instance dle_pfx_preorder : PreOrder dle_pfx.
+      destruct deq_store_equiv as [RS SS TS].
+      split; unfold dle_pfx.
+      - unfold Reflexive.
+        intros.
+        auto using dle_evt_lst_refl.
+      - unfold Transitive.
+        intros [s1 l1] [s2 l2] [s3 l3].
+        simpl.
+        intros [H1 H2] [H3 H4].
+        split.
+        + apply (dle_evt_lst_trans l1 l2 l3); auto.
+        + apply (TS s1 s2 s3); auto.
+    Defined.
+  End DeqTracePfx.
 End SecurityTheory.
